\documentclass[a4paper]{article}

\usepackage[english]{babel}
\usepackage[utf8]{inputenc}
\usepackage{amsmath}
\usepackage{graphicx}
\usepackage{amssymb}
\usepackage{amsthm}
\usepackage{tikz-cd}
\usepackage{mathrsfs}
\usepackage[colorinlistoftodos]{todonotes}
\usepackage{enumitem}
\usepackage{yfonts}


\date{\today}
\newtheorem{thm}{Theorem}[section]
\newtheorem{lem}[thm]{Lemma}

\newtheorem{defn}[thm]{Definition}
\newtheorem{eg}[thm]{Example}
\newtheorem{ex}[thm]{Exercise}
\newtheorem{conj}[thm]{Conjecture}
\newtheorem{cor}[thm]{Corollary}
\newtheorem{claim}[thm]{Claim}
\newtheorem{rmk}[thm]{Remark}

\newcommand{\ie}{\emph{i.e.} }
\newcommand{\cf}{\emph{cf.} }
\newcommand{\into}{\hookrightarrow}
\newcommand{\dirac}{\slashed{\partial}}
\newcommand{\R}{\mathbb{R}}
\newcommand{\C}{\mathbb{C}}
\newcommand{\Z}{\mathbb{Z}}
\newcommand{\N}{\mathbb{N}}
\newcommand{\LieT}{\mathfrak{t}}
\newcommand{\T}{\mathbb{T}}


\begin{document}

According to equation (11) in the paper.

		$$P=\frac{G-\frac{1-\psi}{z}}{\psi/z}=\frac{zG-1+\psi}{\psi}=\frac{z}{\psi}G-\frac{1}{\psi}+1$$

With $\zeta=0$, also WLOG set $\eta=1$, according to equation (12) \& (13) (plug in $t=\frac{1}{z\psi}$):

$$P=1+\frac{1}{z\psi}[1+(P-1)\phi][1+(P-1)\psi]$$

Let $Q=P-1:$

$$Q=P-1 =\frac{z}{\psi} G -\frac{1}{\psi}$$

Rearrange the previous equation:

$$Q\cdot z\psi = (1+Q\phi)(1+Q\psi)=1+Q(\phi+\psi)+Q^2\phi\psi$$

$$\phi\psi Q^2+(\phi+\psi-z\psi)Q+1=0$$

Now plug in $Q$ with $z,\psi,G$:

$$\phi\psi\left(\frac{z^2}{\psi^2}G^2-\frac{2z}{\psi^2}G+\frac1{\psi^2}\right)+\frac{z\phi}{\psi}G+zG-zG-\frac{\phi}{\psi}-1+z+1=0$$

$$\left(\frac{\phi z^2}{\psi}\right)G^2+\left(\frac{z\phi}{\psi}+z-z^2-\frac{2z}{\psi^2}\right)\cdot\phi\psi G+\frac{\phi}{\psi}-\frac{\phi}{\psi}-1+1+z=0$$

$$\frac{\phi z^2}{\psi}G^2+\left(z[1-\frac{\phi}{\psi}-z]\right)G+z=0\ \ \ (\star)$$

$(\star)$ times $\frac{\psi}{\phi z}$ to generate our target equation:

$$zG^2+\left(\frac{\psi}{\phi}-1-\frac{z\psi}{\phi}\right)G+\frac{\psi}{\phi} = 0$$

$$zG^2+\left((1-z)\frac{\psi}{\phi}-1\right)G+\frac{\psi}{\phi} = 0$$

Here we have something ``strange", as the our desired equation is

$$zG^2+\left((1-\frac{\psi}{\phi})z-1\right)G+\frac{\psi}{\phi}=0$$

Is it a possible typo?
\end{document}
